feat: data_create_s1_el1

container/coq/pointer/.CachedSpec/Layer8Spec.v
@@ -36,20 +36,195 @@ Definition rtt_create_s1_el1_spec_abs (v_0: Ptr) (v_1: abs_PA_t) (v_2: Z) (v_3: 
   when v_7, st_2 == ((rtt_create_internal_spec_abs ttbr v_1 v_2 v_3 1 st_1));
   ((Some v_7), st_2).
 
-Definition update_ripas_spec (v_0: Ptr) (v_1: Z) (v_2: Z) (st: RData) : (option (bool * RData)) :=
-  if ((v_1 <? (3)) && ((((test_Ptr_PTE v_0).(meta_desc_type)) =? (3))))
-  then (Some (false, st))
+Definition data_create_s1_el1_0 (st_0: RData) (st_7: RData) (v_25: Z) (ret_1: Ptr) (ret_2: Ptr) : (option (Z * RData)) :=
+  let v_29 := ret_2 in
+  when st_10 == ((granule_unlock_spec v_29 st_7));
+  let v_30 := ret_1 in
+  when st_12 == ((granule_unlock_transition_spec v_30 4 st_10));
+  when st_15 == ((free_stack "data_create_s1_el1" st_0 st_12));
+  (Some (v_25, st_15)).
+
+Definition data_create_s1_el1_spec (v_0: Z) (v_1: Z) (v_2: Z) (v_3: Ptr) (st: RData) : (option (Z * RData)) :=
+  rely (((((v_3.(pbase)) = ("granules")) /\ ((((v_3.(poffset)) mod (16)) = (0)))) /\ (((v_3.(poffset)) >= (0)))));
+  if (((((test_Z_PTE v_0).(meta_PA)).(meta_granule_offset)) - (((test_PA v_1).(meta_granule_offset)))) =? (0))
+  then (Some ((pack_struct_return_code_para (make_return_code_para 3)), st))
   else (
-    if ((v_1 =? (3)) && ((((test_Ptr_PTE v_0).(meta_desc_type)) =? (3))))
-    then (Some (true, st))
-    else (
-      if ((v_1 <>? (3)) && ((((test_Ptr_PTE v_0).(meta_desc_type)) =? (1))))
-      then (Some (true, st))
-      else (
-        if (((((test_Ptr_PTE v_0).(meta_desc_type)) =? (0)) && ((((test_Ptr_PTE v_0).(meta_ripas)) =? (0)))) && ((((test_Ptr_PTE v_0).(meta_mem_attr)) =? (0))))
-        then (Some (true, st))
+    when st_1 == ((spinlock_acquire_spec (mkPtr "granules" (((test_Z_PTE v_0).(meta_PA)).(meta_granule_offset))) st));
+    if (((((((st_1.(share)).(globals)).(g_granules)) @ ((((test_Z_PTE v_0).(meta_PA)).(meta_granule_offset)) / (16))).(e_state_s_granule)) - (1)) =? (0))
+    then (
+      when st_2 == ((spinlock_acquire_spec (mkPtr "granules" ((test_PA v_1).(meta_granule_offset))) st_1));
+      if (((((((st_2.(share)).(globals)).(g_granules)) @ (((test_PA v_1).(meta_granule_offset)) / (16))).(e_state_s_granule)) - (3)) =? (0))
+      then (
+        when st_6 == ((granule_lock_spec (rec_to_ttbr1_para (mkPtr "granule_data" ((test_PA v_1).(meta_granule_offset))) st_2) 5 st_2));
+        rely (((((((st_6.(share)).(granule_data)) @ (((test_PA v_1).(meta_granule_offset)) / (4096))).(g_granule_state)) - (GRANULE_STATE_REC)) = (0)));
+        rely (((("granule_data" = ("granule_data")) /\ (((((test_PA v_1).(meta_granule_offset)) mod (4096)) = (0)))) /\ ((((test_PA v_1).(meta_granule_offset)) >= (0)))));
+        when rtt_ret, st_4 == (
+            (rtt_walk_lock_unlock_spec_abs
+              (mkPtr "stack_s_rtt_walk" 0)
+              (rec_to_ttbr1_para (mkPtr "granule_data" ((test_PA v_1).(meta_granule_offset))) st_2)
+              0
+              64
+              v_2
+              3
+              st_6));
+        rely ((((st_4.(share)).(granule_data)) = (((st_6.(share)).(granule_data)))));
+        if ((rtt_ret.(e_1)) =? (3))
+        then (
+          if (
+            (((((abs_tte_read (mkPtr "granule_data" (((rtt_ret.(e_2)).(poffset)) + ((8 * ((rtt_ret.(e_3))))))) st_4).(meta_desc_type)) =? (0)) &&
+              ((((abs_tte_read (mkPtr "granule_data" (((rtt_ret.(e_2)).(poffset)) + ((8 * ((rtt_ret.(e_3))))))) st_4).(meta_ripas)) =? (0)))) &&
+              ((((abs_tte_read (mkPtr "granule_data" (((rtt_ret.(e_2)).(poffset)) + ((8 * ((rtt_ret.(e_3))))))) st_4).(meta_mem_attr)) =? (0)))))
+          then (
+            when st_13 == ((granule_lock_spec (rec_to_rd_para (mkPtr "granule_data" ((test_PA v_1).(meta_granule_offset))) st_4) 2 st_4));
+            when v_11, st_3 == ((memcpy_ns_read_spec (mkPtr "granule_data" (((test_Z_PTE v_0).(meta_PA)).(meta_granule_offset))) (mkPtr "granule_data" (v_3.(poffset))) 4096 st_13));
+            if v_11
+            then (
+              when st_18 == ((granule_unlock_spec (rec_to_rd_para (mkPtr "granule_data" ((test_PA v_1).(meta_granule_offset))) st_4) st_3));
+              rely ((((rtt_ret.(e_2)).(pbase)) =s ("granules")));
+              rely ((((((rtt_ret.(e_2)).(poffset)) + (8)) mod (16)) = (8)));
+              rely (
+                ((("granules" = ("granules")) /\ ((((((test_Z_PTE v_0).(meta_PA)).(meta_granule_offset)) mod (16)) = (0)))) /\
+                  (((((test_Z_PTE v_0).(meta_PA)).(meta_granule_offset)) >= (0)))));
+              if (((((((test_Z_PTE v_0).(meta_PA)).(meta_granule_offset)) + (8)) mod (16)) - (8)) =? (0))
+              then (
+                when st_30 == (
+                    (granule_unlock_spec
+                      (rtt_ret.(e_2))
+                      ((st_18.[share].[globals].[g_granules] :<
+                        (((((st_18.(share)).(globals)).(g_granules)) #
+                          ((((rtt_ret.(e_2)).(poffset)) + (8)) / (16)) ==
+                          (((((st_18.(share)).(globals)).(g_granules)) @ ((((rtt_ret.(e_2)).(poffset)) + (8)) / (16))).[e_ref] :<
+                            ((((((st_18.(share)).(globals)).(g_granules)) @ ((((rtt_ret.(e_2)).(poffset)) + (8)) / (16))).(e_ref)).[e_u_anon_3_0] :<
+                              (((((((st_18.(share)).(globals)).(g_granules)) @ ((((rtt_ret.(e_2)).(poffset)) + (8)) / (16))).(e_ref)).(e_u_anon_3_0)) + (1))))) #
+                          ((((test_Z_PTE v_0).(meta_PA)).(meta_granule_offset)) / (16)) ==
+                          ((((((st_18.(share)).(globals)).(g_granules)) #
+                            ((((rtt_ret.(e_2)).(poffset)) + (8)) / (16)) ==
+                            (((((st_18.(share)).(globals)).(g_granules)) @ ((((rtt_ret.(e_2)).(poffset)) + (8)) / (16))).[e_ref] :<
+                              ((((((st_18.(share)).(globals)).(g_granules)) @ ((((rtt_ret.(e_2)).(poffset)) + (8)) / (16))).(e_ref)).[e_u_anon_3_0] :<
+                                (((((((st_18.(share)).(globals)).(g_granules)) @ ((((rtt_ret.(e_2)).(poffset)) + (8)) / (16))).(e_ref)).(e_u_anon_3_0)) + (1))))) @ ((((test_Z_PTE v_0).(meta_PA)).(meta_granule_offset)) / (16))).[e_ref] :<
+                            (((((((st_18.(share)).(globals)).(g_granules)) #
+                              ((((rtt_ret.(e_2)).(poffset)) + (8)) / (16)) ==
+                              (((((st_18.(share)).(globals)).(g_granules)) @ ((((rtt_ret.(e_2)).(poffset)) + (8)) / (16))).[e_ref] :<
+                                ((((((st_18.(share)).(globals)).(g_granules)) @ ((((rtt_ret.(e_2)).(poffset)) + (8)) / (16))).(e_ref)).[e_u_anon_3_0] :<
+                                  (((((((st_18.(share)).(globals)).(g_granules)) @ ((((rtt_ret.(e_2)).(poffset)) + (8)) / (16))).(e_ref)).(e_u_anon_3_0)) + (1))))) @ ((((test_Z_PTE v_0).(meta_PA)).(meta_granule_offset)) / (16))).(e_ref)).[e_u_anon_3_0] :<
+                              ((g_mapped_addr_set_para
+                                (((((((st_18.(share)).(globals)).(g_granules)) #
+                                  ((((rtt_ret.(e_2)).(poffset)) + (8)) / (16)) ==
+                                  (((((st_18.(share)).(globals)).(g_granules)) @ ((((rtt_ret.(e_2)).(poffset)) + (8)) / (16))).[e_ref] :<
+                                    ((((((st_18.(share)).(globals)).(g_granules)) @ ((((rtt_ret.(e_2)).(poffset)) + (8)) / (16))).(e_ref)).[e_u_anon_3_0] :<
+                                      (((((((st_18.(share)).(globals)).(g_granules)) @ ((((rtt_ret.(e_2)).(poffset)) + (8)) / (16))).(e_ref)).(e_u_anon_3_0)) + (1))))) @ ((((test_Z_PTE v_0).(meta_PA)).(meta_granule_offset)) / (16))).(e_ref)).(e_u_anon_3_0))
+                                v_2) +
+                                (1)))))).[share].[granule_data] :<
+                        (((st_18.(share)).(granule_data)) #
+                          ((((rtt_ret.(e_2)).(poffset)) + ((8 * ((rtt_ret.(e_3)))))) / (4096)) ==
+                          ((((st_18.(share)).(granule_data)) @ ((((rtt_ret.(e_2)).(poffset)) + ((8 * ((rtt_ret.(e_3)))))) / (4096))).[g_norm] :<
+                            (((((st_18.(share)).(granule_data)) @ ((((rtt_ret.(e_2)).(poffset)) + ((8 * ((rtt_ret.(e_3)))))) / (4096))).(g_norm)) #
+                              ((((rtt_ret.(e_2)).(poffset)) + ((8 * ((rtt_ret.(e_3)))))) mod (4096)) ==
+                              (test_PTE_Z (mkabs_PTE_t ((test_Z_PTE v_0).(meta_PA)) 0 0 3))))))));
+                when st_10 == ((granule_unlock_spec (mkPtr "granules" ((test_PA v_1).(meta_granule_offset))) st_30));
+                when st_5 == (
+                    (granule_unlock_spec
+                      (mkPtr "granules" (((test_Z_PTE v_0).(meta_PA)).(meta_granule_offset)))
+                      (st_10.[share].[globals].[g_granules] :<
+                        ((((st_10.(share)).(globals)).(g_granules)) #
+                          ((((test_Z_PTE v_0).(meta_PA)).(meta_granule_offset)) / (16)) ==
+                          (((((st_10.(share)).(globals)).(g_granules)) @ ((((test_Z_PTE v_0).(meta_PA)).(meta_granule_offset)) / (16))).[e_state_s_granule] :< 4)))));
+                (Some (0, st_5)))
+              else None)
+            else (
+              when v_33, st_18 == ((memset_spec (mkPtr "granule_data" (((test_Z_PTE v_0).(meta_PA)).(meta_granule_offset))) 0 4096 st_3));
+              when st_19 == ((granule_unlock_spec (rec_to_rd_para (mkPtr "granule_data" ((test_PA v_1).(meta_granule_offset))) st_4) st_18));
+              when st_21 == ((granule_unlock_spec (rtt_ret.(e_2)) st_19));
+              if ((pack_struct_return_code_para (make_return_code_para 1)) =? (0))
+              then (
+                when st_10 == ((granule_unlock_spec (mkPtr "granules" ((test_PA v_1).(meta_granule_offset))) st_21));
+                rely (
+                  ((("granules" = ("granules")) /\ ((((((test_Z_PTE v_0).(meta_PA)).(meta_granule_offset)) mod (16)) = (0)))) /\
+                    (((((test_Z_PTE v_0).(meta_PA)).(meta_granule_offset)) >= (0)))));
+                when st_5 == (
+                    (granule_unlock_spec
+                      (mkPtr "granules" (((test_Z_PTE v_0).(meta_PA)).(meta_granule_offset)))
+                      (st_10.[share].[globals].[g_granules] :<
+                        ((((st_10.(share)).(globals)).(g_granules)) #
+                          ((((test_Z_PTE v_0).(meta_PA)).(meta_granule_offset)) / (16)) ==
+                          (((((st_10.(share)).(globals)).(g_granules)) @ ((((test_Z_PTE v_0).(meta_PA)).(meta_granule_offset)) / (16))).[e_state_s_granule] :< 4)))));
+                (Some ((pack_struct_return_code_para (make_return_code_para 1)), st_5)))
+              else (
+                when st_10 == ((granule_unlock_spec (mkPtr "granules" ((test_PA v_1).(meta_granule_offset))) st_21));
+                rely (
+                  ((("granules" = ("granules")) /\ ((((((test_Z_PTE v_0).(meta_PA)).(meta_granule_offset)) mod (16)) = (0)))) /\
+                    (((((test_Z_PTE v_0).(meta_PA)).(meta_granule_offset)) >= (0)))));
+                when st_5 == (
+                    (granule_unlock_spec
+                      (mkPtr "granules" (((test_Z_PTE v_0).(meta_PA)).(meta_granule_offset)))
+                      (st_10.[share].[globals].[g_granules] :<
+                        ((((st_10.(share)).(globals)).(g_granules)) #
+                          ((((test_Z_PTE v_0).(meta_PA)).(meta_granule_offset)) / (16)) ==
+                          (((((st_10.(share)).(globals)).(g_granules)) @ ((((test_Z_PTE v_0).(meta_PA)).(meta_granule_offset)) / (16))).[e_state_s_granule] :< 1)))));
+                (Some ((pack_struct_return_code_para (make_return_code_para 1)), st_5)))))
+          else (
+            when st_13 == ((granule_unlock_spec (rtt_ret.(e_2)) st_4));
+            if ((pack_struct_return_code_para (make_return_code_para 9)) =? (0))
+            then (
+              when st_10 == ((granule_unlock_spec (mkPtr "granules" ((test_PA v_1).(meta_granule_offset))) st_13));
+              rely (
+                ((("granules" = ("granules")) /\ ((((((test_Z_PTE v_0).(meta_PA)).(meta_granule_offset)) mod (16)) = (0)))) /\
+                  (((((test_Z_PTE v_0).(meta_PA)).(meta_granule_offset)) >= (0)))));
+              when st_3 == (
+                  (granule_unlock_spec
+                    (mkPtr "granules" (((test_Z_PTE v_0).(meta_PA)).(meta_granule_offset)))
+                    (st_10.[share].[globals].[g_granules] :<
+                      ((((st_10.(share)).(globals)).(g_granules)) #
+                        ((((test_Z_PTE v_0).(meta_PA)).(meta_granule_offset)) / (16)) ==
+                        (((((st_10.(share)).(globals)).(g_granules)) @ ((((test_Z_PTE v_0).(meta_PA)).(meta_granule_offset)) / (16))).[e_state_s_granule] :< 4)))));
+              (Some ((pack_struct_return_code_para (make_return_code_para 9)), st_3)))
+            else (
+              when st_10 == ((granule_unlock_spec (mkPtr "granules" ((test_PA v_1).(meta_granule_offset))) st_13));
+              rely (
+                ((("granules" = ("granules")) /\ ((((((test_Z_PTE v_0).(meta_PA)).(meta_granule_offset)) mod (16)) = (0)))) /\
+                  (((((test_Z_PTE v_0).(meta_PA)).(meta_granule_offset)) >= (0)))));
+              when st_3 == (
+                  (granule_unlock_spec
+                    (mkPtr "granules" (((test_Z_PTE v_0).(meta_PA)).(meta_granule_offset)))
+                    (st_10.[share].[globals].[g_granules] :<
+                      ((((st_10.(share)).(globals)).(g_granules)) #
+                        ((((test_Z_PTE v_0).(meta_PA)).(meta_granule_offset)) / (16)) ==
+                        (((((st_10.(share)).(globals)).(g_granules)) @ ((((test_Z_PTE v_0).(meta_PA)).(meta_granule_offset)) / (16))).[e_state_s_granule] :< 1)))));
+              (Some ((pack_struct_return_code_para (make_return_code_para 9)), st_3)))))
         else (
-          if (((((test_Ptr_PTE v_0).(meta_desc_type)) =? (0)) && ((((test_Ptr_PTE v_0).(meta_ripas)) =? (0)))) && ((((test_Ptr_PTE v_0).(meta_mem_attr)) =? (1))))
-          then (Some (true, st))
-          else (Some (false, st)))))).
+          when st_8 == ((granule_unlock_spec (rtt_ret.(e_2)) st_4));
+          if ((pack_struct_return_code_para (make_return_code_para 8)) =? (0))
+          then (
+            when st_10 == ((granule_unlock_spec (mkPtr "granules" ((test_PA v_1).(meta_granule_offset))) st_8));
+            rely (
+              ((("granules" = ("granules")) /\ ((((((test_Z_PTE v_0).(meta_PA)).(meta_granule_offset)) mod (16)) = (0)))) /\
+                (((((test_Z_PTE v_0).(meta_PA)).(meta_granule_offset)) >= (0)))));
+            when st_3 == (
+                (granule_unlock_spec
+                  (mkPtr "granules" (((test_Z_PTE v_0).(meta_PA)).(meta_granule_offset)))
+                  (st_10.[share].[globals].[g_granules] :<
+                    ((((st_10.(share)).(globals)).(g_granules)) #
+                      ((((test_Z_PTE v_0).(meta_PA)).(meta_granule_offset)) / (16)) ==
+                      (((((st_10.(share)).(globals)).(g_granules)) @ ((((test_Z_PTE v_0).(meta_PA)).(meta_granule_offset)) / (16))).[e_state_s_granule] :< 4)))));
+            (Some ((pack_struct_return_code_para (make_return_code_para 8)), st_3)))
+          else (
+            when st_10 == ((granule_unlock_spec (mkPtr "granules" ((test_PA v_1).(meta_granule_offset))) st_8));
+            rely (
+              ((("granules" = ("granules")) /\ ((((((test_Z_PTE v_0).(meta_PA)).(meta_granule_offset)) mod (16)) = (0)))) /\
+                (((((test_Z_PTE v_0).(meta_PA)).(meta_granule_offset)) >= (0)))));
+            when st_3 == (
+                (granule_unlock_spec
+                  (mkPtr "granules" (((test_Z_PTE v_0).(meta_PA)).(meta_granule_offset)))
+                  (st_10.[share].[globals].[g_granules] :<
+                    ((((st_10.(share)).(globals)).(g_granules)) #
+                      ((((test_Z_PTE v_0).(meta_PA)).(meta_granule_offset)) / (16)) ==
+                      (((((st_10.(share)).(globals)).(g_granules)) @ ((((test_Z_PTE v_0).(meta_PA)).(meta_granule_offset)) / (16))).[e_state_s_granule] :< 1)))));
+            (Some ((pack_struct_return_code_para (make_return_code_para 8)), st_3)))))
+      else (
+        when st_3 == ((spinlock_release_spec (mkPtr "granules" ((test_PA v_1).(meta_granule_offset))) st_2));
+        when st_4 == ((granule_unlock_spec (mkPtr "granules" (((test_Z_PTE v_0).(meta_PA)).(meta_granule_offset))) st_3));
+        (Some ((pack_struct_return_code_para (make_return_code_para 3)), st_4))))
+    else (
+      when st_2 == ((spinlock_release_spec (mkPtr "granules" (((test_Z_PTE v_0).(meta_PA)).(meta_granule_offset))) st_1));
+      (Some ((pack_struct_return_code_para (make_return_code_para 3)), st_2)))).
 
