container/coq/pointer/Layer7/Spec.v
@@ -351,171 +351,7 @@ Section Layer7_Spec.
     when v_6, st_1 == ((memcpy_ns_read_spec v_3 v_5 v_2 st_0));
     (Some (v_6, st_1)).
 
-  Definition data_create_internal_0 (st_0: RData) (st_14: RData) (v_18: Ptr) (v_2: Z) (v_41: abs_PTE_t) (v_5: Z) (v_9: Ptr) (v__sroa_0_0_copyload: Ptr) (v__sroa_4_0_copyload: Z) : (option (Z * RData)) :=
-    rely (((v_5 =? (0)) = (true)));
-    rely (((v__sroa_0_0_copyload.(pbase)) =s ("granules")));
-    rely (((((v__sroa_0_0_copyload.(poffset)) + (8)) mod (16)) = (8)));
-    rely (((((v_9.(pbase)) = ("granules")) /\ ((((v_9.(poffset)) mod (16)) = (0)))) /\ (((v_9.(poffset)) >= (0)))));
-    when st_24 == (
-        (granule_unlock_spec
-          v__sroa_0_0_copyload
-          ((st_14.[share].[globals].[g_granules] :<
-            (((((st_14.(share)).(globals)).(g_granules)) #
-              (((v__sroa_0_0_copyload.(poffset)) + (8)) / (16)) ==
-              (((((st_14.(share)).(globals)).(g_granules)) @ (((v__sroa_0_0_copyload.(poffset)) + (8)) / (16))).[e_ref] :<
-                ((((((st_14.(share)).(globals)).(g_granules)) @ (((v__sroa_0_0_copyload.(poffset)) + (8)) / (16))).(e_ref)).[e_u_anon_3_0] :<
-                  (((((((st_14.(share)).(globals)).(g_granules)) @ (((v__sroa_0_0_copyload.(poffset)) + (8)) / (16))).(e_ref)).(e_u_anon_3_0)) + (1))))) #
-              ((v_9.(poffset)) / (16)) ==
-              ((((((st_14.(share)).(globals)).(g_granules)) #
-                (((v__sroa_0_0_copyload.(poffset)) + (8)) / (16)) ==
-                (((((st_14.(share)).(globals)).(g_granules)) @ (((v__sroa_0_0_copyload.(poffset)) + (8)) / (16))).[e_ref] :<
-                  ((((((st_14.(share)).(globals)).(g_granules)) @ (((v__sroa_0_0_copyload.(poffset)) + (8)) / (16))).(e_ref)).[e_u_anon_3_0] :<
-                    (((((((st_14.(share)).(globals)).(g_granules)) @ (((v__sroa_0_0_copyload.(poffset)) + (8)) / (16))).(e_ref)).(e_u_anon_3_0)) + (1))))) @ ((v_9.(poffset)) / (16))).[e_ref] :<
-                (((((((st_14.(share)).(globals)).(g_granules)) #
-                  (((v__sroa_0_0_copyload.(poffset)) + (8)) / (16)) ==
-                  (((((st_14.(share)).(globals)).(g_granules)) @ (((v__sroa_0_0_copyload.(poffset)) + (8)) / (16))).[e_ref] :<
-                    ((((((st_14.(share)).(globals)).(g_granules)) @ (((v__sroa_0_0_copyload.(poffset)) + (8)) / (16))).(e_ref)).[e_u_anon_3_0] :<
-                      (((((((st_14.(share)).(globals)).(g_granules)) @ (((v__sroa_0_0_copyload.(poffset)) + (8)) / (16))).(e_ref)).(e_u_anon_3_0)) + (1))))) @ ((v_9.(poffset)) / (16))).(e_ref)).[e_u_anon_3_0] :<
-                  ((g_mapped_addr_set_para
-                    (((((((st_14.(share)).(globals)).(g_granules)) #
-                      (((v__sroa_0_0_copyload.(poffset)) + (8)) / (16)) ==
-                      (((((st_14.(share)).(globals)).(g_granules)) @ (((v__sroa_0_0_copyload.(poffset)) + (8)) / (16))).[e_ref] :<
-                        ((((((st_14.(share)).(globals)).(g_granules)) @ (((v__sroa_0_0_copyload.(poffset)) + (8)) / (16))).(e_ref)).[e_u_anon_3_0] :<
-                          (((((((st_14.(share)).(globals)).(g_granules)) @ (((v__sroa_0_0_copyload.(poffset)) + (8)) / (16))).(e_ref)).(e_u_anon_3_0)) + (1))))) @ ((v_9.(poffset)) / (16))).(e_ref)).(e_u_anon_3_0))
-                    v_2) +
-                    (1)))))).[share].[granule_data] :<
-            (((st_14.(share)).(granule_data)) #
-              (((v_18.(poffset)) + ((8 * (v__sroa_4_0_copyload)))) / (4096)) ==
-              ((((st_14.(share)).(granule_data)) @ (((v_18.(poffset)) + ((8 * (v__sroa_4_0_copyload)))) / (4096))).[g_norm] :<
-                (((((st_14.(share)).(granule_data)) @ (((v_18.(poffset)) + ((8 * (v__sroa_4_0_copyload)))) / (4096))).(g_norm)) #
-                  (((v_18.(poffset)) + ((8 * (v__sroa_4_0_copyload)))) mod (4096)) ==
-                  (test_PTE_Z v_41)))))));
-    (Some (0, st_24)).
-
-  Definition data_create_internal_1 (st_0: RData) (st_13: RData) (v_0: abs_PTE_t) (v_18: Ptr) (v_2: Z) (v_5: Z) (v_9: Ptr) (v__sroa_0_0_copyload: Ptr) (v__sroa_4_0_copyload: Z) : (option (Z * RData)) :=
-    rely (((v_5 =? (0)) = (true)));
-    rely (((v__sroa_0_0_copyload.(pbase)) =s ("granules")));
-    rely (((((v__sroa_0_0_copyload.(poffset)) + (8)) mod (16)) = (8)));
-    rely (((((v_9.(pbase)) = ("granules")) /\ ((((v_9.(poffset)) mod (16)) = (0)))) /\ (((v_9.(poffset)) >= (0)))));
-    when st_23 == (
-        (granule_unlock_spec
-          v__sroa_0_0_copyload
-          ((st_13.[share].[globals].[g_granules] :<
-            (((((st_13.(share)).(globals)).(g_granules)) #
-              (((v__sroa_0_0_copyload.(poffset)) + (8)) / (16)) ==
-              (((((st_13.(share)).(globals)).(g_granules)) @ (((v__sroa_0_0_copyload.(poffset)) + (8)) / (16))).[e_ref] :<
-                ((((((st_13.(share)).(globals)).(g_granules)) @ (((v__sroa_0_0_copyload.(poffset)) + (8)) / (16))).(e_ref)).[e_u_anon_3_0] :<
-                  (((((((st_13.(share)).(globals)).(g_granules)) @ (((v__sroa_0_0_copyload.(poffset)) + (8)) / (16))).(e_ref)).(e_u_anon_3_0)) + (1))))) #
-              ((v_9.(poffset)) / (16)) ==
-              ((((((st_13.(share)).(globals)).(g_granules)) #
-                (((v__sroa_0_0_copyload.(poffset)) + (8)) / (16)) ==
-                (((((st_13.(share)).(globals)).(g_granules)) @ (((v__sroa_0_0_copyload.(poffset)) + (8)) / (16))).[e_ref] :<
-                  ((((((st_13.(share)).(globals)).(g_granules)) @ (((v__sroa_0_0_copyload.(poffset)) + (8)) / (16))).(e_ref)).[e_u_anon_3_0] :<
-                    (((((((st_13.(share)).(globals)).(g_granules)) @ (((v__sroa_0_0_copyload.(poffset)) + (8)) / (16))).(e_ref)).(e_u_anon_3_0)) + (1))))) @ ((v_9.(poffset)) / (16))).[e_ref] :<
-                (((((((st_13.(share)).(globals)).(g_granules)) #
-                  (((v__sroa_0_0_copyload.(poffset)) + (8)) / (16)) ==
-                  (((((st_13.(share)).(globals)).(g_granules)) @ (((v__sroa_0_0_copyload.(poffset)) + (8)) / (16))).[e_ref] :<
-                    ((((((st_13.(share)).(globals)).(g_granules)) @ (((v__sroa_0_0_copyload.(poffset)) + (8)) / (16))).(e_ref)).[e_u_anon_3_0] :<
-                      (((((((st_13.(share)).(globals)).(g_granules)) @ (((v__sroa_0_0_copyload.(poffset)) + (8)) / (16))).(e_ref)).(e_u_anon_3_0)) + (1))))) @ ((v_9.(poffset)) / (16))).(e_ref)).[e_u_anon_3_0] :<
-                  ((g_mapped_addr_set_para
-                    (((((((st_13.(share)).(globals)).(g_granules)) #
-                      (((v__sroa_0_0_copyload.(poffset)) + (8)) / (16)) ==
-                      (((((st_13.(share)).(globals)).(g_granules)) @ (((v__sroa_0_0_copyload.(poffset)) + (8)) / (16))).[e_ref] :<
-                        ((((((st_13.(share)).(globals)).(g_granules)) @ (((v__sroa_0_0_copyload.(poffset)) + (8)) / (16))).(e_ref)).[e_u_anon_3_0] :<
-                          (((((((st_13.(share)).(globals)).(g_granules)) @ (((v__sroa_0_0_copyload.(poffset)) + (8)) / (16))).(e_ref)).(e_u_anon_3_0)) + (1))))) @ ((v_9.(poffset)) / (16))).(e_ref)).(e_u_anon_3_0))
-                    v_2) +
-                    (1)))))).[share].[granule_data] :<
-            (((st_13.(share)).(granule_data)) #
-              (((v_18.(poffset)) + ((8 * (v__sroa_4_0_copyload)))) / (4096)) ==
-              ((((st_13.(share)).(granule_data)) @ (((v_18.(poffset)) + ((8 * (v__sroa_4_0_copyload)))) / (4096))).[g_norm] :<
-                (((((st_13.(share)).(granule_data)) @ (((v_18.(poffset)) + ((8 * (v__sroa_4_0_copyload)))) / (4096))).(g_norm)) #
-                  (((v_18.(poffset)) + ((8 * (v__sroa_4_0_copyload)))) mod (4096)) ==
-                  (test_PTE_Z v_0)))))));
-    (Some (0, st_23)).
-
-  Definition data_create_internal_2 (st_0: RData) (st_21: RData) (v_18: Ptr) (v_2: Z) (v_41: abs_PTE_t) (v_5: Z) (v_9: Ptr) (v__sroa_0_0_copyload: Ptr) (v__sroa_4_0_copyload: Z) : (option (Z * RData)) :=
-    rely (((v_5 =? (0)) = (true)));
-    rely (((v__sroa_0_0_copyload.(pbase)) =s ("granules")));
-    rely (((((v__sroa_0_0_copyload.(poffset)) + (8)) mod (16)) = (8)));
-    rely (((((v_9.(pbase)) = ("granules")) /\ ((((v_9.(poffset)) mod (16)) = (0)))) /\ (((v_9.(poffset)) >= (0)))));
-    when st_29 == (
-        (granule_unlock_spec
-          v__sroa_0_0_copyload
-          ((st_21.[share].[globals].[g_granules] :<
-            (((((st_21.(share)).(globals)).(g_granules)) #
-              (((v__sroa_0_0_copyload.(poffset)) + (8)) / (16)) ==
-              (((((st_21.(share)).(globals)).(g_granules)) @ (((v__sroa_0_0_copyload.(poffset)) + (8)) / (16))).[e_ref] :<
-                ((((((st_21.(share)).(globals)).(g_granules)) @ (((v__sroa_0_0_copyload.(poffset)) + (8)) / (16))).(e_ref)).[e_u_anon_3_0] :<
-                  (((((((st_21.(share)).(globals)).(g_granules)) @ (((v__sroa_0_0_copyload.(poffset)) + (8)) / (16))).(e_ref)).(e_u_anon_3_0)) + (1))))) #
-              ((v_9.(poffset)) / (16)) ==
-              ((((((st_21.(share)).(globals)).(g_granules)) #
-                (((v__sroa_0_0_copyload.(poffset)) + (8)) / (16)) ==
-                (((((st_21.(share)).(globals)).(g_granules)) @ (((v__sroa_0_0_copyload.(poffset)) + (8)) / (16))).[e_ref] :<
-                  ((((((st_21.(share)).(globals)).(g_granules)) @ (((v__sroa_0_0_copyload.(poffset)) + (8)) / (16))).(e_ref)).[e_u_anon_3_0] :<
-                    (((((((st_21.(share)).(globals)).(g_granules)) @ (((v__sroa_0_0_copyload.(poffset)) + (8)) / (16))).(e_ref)).(e_u_anon_3_0)) + (1))))) @ ((v_9.(poffset)) / (16))).[e_ref] :<
-                (((((((st_21.(share)).(globals)).(g_granules)) #
-                  (((v__sroa_0_0_copyload.(poffset)) + (8)) / (16)) ==
-                  (((((st_21.(share)).(globals)).(g_granules)) @ (((v__sroa_0_0_copyload.(poffset)) + (8)) / (16))).[e_ref] :<
-                    ((((((st_21.(share)).(globals)).(g_granules)) @ (((v__sroa_0_0_copyload.(poffset)) + (8)) / (16))).(e_ref)).[e_u_anon_3_0] :<
-                      (((((((st_21.(share)).(globals)).(g_granules)) @ (((v__sroa_0_0_copyload.(poffset)) + (8)) / (16))).(e_ref)).(e_u_anon_3_0)) + (1))))) @ ((v_9.(poffset)) / (16))).(e_ref)).[e_u_anon_3_0] :<
-                  ((g_mapped_addr_set_para
-                    (((((((st_21.(share)).(globals)).(g_granules)) #
-                      (((v__sroa_0_0_copyload.(poffset)) + (8)) / (16)) ==
-                      (((((st_21.(share)).(globals)).(g_granules)) @ (((v__sroa_0_0_copyload.(poffset)) + (8)) / (16))).[e_ref] :<
-                        ((((((st_21.(share)).(globals)).(g_granules)) @ (((v__sroa_0_0_copyload.(poffset)) + (8)) / (16))).(e_ref)).[e_u_anon_3_0] :<
-                          (((((((st_21.(share)).(globals)).(g_granules)) @ (((v__sroa_0_0_copyload.(poffset)) + (8)) / (16))).(e_ref)).(e_u_anon_3_0)) + (1))))) @ ((v_9.(poffset)) / (16))).(e_ref)).(e_u_anon_3_0))
-                    v_2) +
-                    (1)))))).[share].[granule_data] :<
-            (((st_21.(share)).(granule_data)) #
-              (((v_18.(poffset)) + ((8 * (v__sroa_4_0_copyload)))) / (4096)) ==
-              ((((st_21.(share)).(granule_data)) @ (((v_18.(poffset)) + ((8 * (v__sroa_4_0_copyload)))) / (4096))).[g_norm] :<
-                (((((st_21.(share)).(granule_data)) @ (((v_18.(poffset)) + ((8 * (v__sroa_4_0_copyload)))) / (4096))).(g_norm)) #
-                  (((v_18.(poffset)) + ((8 * (v__sroa_4_0_copyload)))) mod (4096)) ==
-                  (test_PTE_Z v_41)))))));
-    (Some (0, st_29)).
-
-  Definition data_create_internal_3 (st_0: RData) (st_20: RData) (v_0: abs_PTE_t) (v_18: Ptr) (v_2: Z) (v_5: Z) (v_9: Ptr) (v__sroa_0_0_copyload: Ptr) (v__sroa_4_0_copyload: Z) : (option (Z * RData)) :=
-    rely (((v_5 =? (0)) = (true)));
-    rely (((v__sroa_0_0_copyload.(pbase)) =s ("granules")));
-    rely (((((v__sroa_0_0_copyload.(poffset)) + (8)) mod (16)) = (8)));
-    rely (((((v_9.(pbase)) = ("granules")) /\ ((((v_9.(poffset)) mod (16)) = (0)))) /\ (((v_9.(poffset)) >= (0)))));
-    when st_28 == (
-        (granule_unlock_spec
-          v__sroa_0_0_copyload
-          ((st_20.[share].[globals].[g_granules] :<
-            (((((st_20.(share)).(globals)).(g_granules)) #
-              (((v__sroa_0_0_copyload.(poffset)) + (8)) / (16)) ==
-              (((((st_20.(share)).(globals)).(g_granules)) @ (((v__sroa_0_0_copyload.(poffset)) + (8)) / (16))).[e_ref] :<
-                ((((((st_20.(share)).(globals)).(g_granules)) @ (((v__sroa_0_0_copyload.(poffset)) + (8)) / (16))).(e_ref)).[e_u_anon_3_0] :<
-                  (((((((st_20.(share)).(globals)).(g_granules)) @ (((v__sroa_0_0_copyload.(poffset)) + (8)) / (16))).(e_ref)).(e_u_anon_3_0)) + (1))))) #
-              ((v_9.(poffset)) / (16)) ==
-              ((((((st_20.(share)).(globals)).(g_granules)) #
-                (((v__sroa_0_0_copyload.(poffset)) + (8)) / (16)) ==
-                (((((st_20.(share)).(globals)).(g_granules)) @ (((v__sroa_0_0_copyload.(poffset)) + (8)) / (16))).[e_ref] :<
-                  ((((((st_20.(share)).(globals)).(g_granules)) @ (((v__sroa_0_0_copyload.(poffset)) + (8)) / (16))).(e_ref)).[e_u_anon_3_0] :<
-                    (((((((st_20.(share)).(globals)).(g_granules)) @ (((v__sroa_0_0_copyload.(poffset)) + (8)) / (16))).(e_ref)).(e_u_anon_3_0)) + (1))))) @ ((v_9.(poffset)) / (16))).[e_ref] :<
-                (((((((st_20.(share)).(globals)).(g_granules)) #
-                  (((v__sroa_0_0_copyload.(poffset)) + (8)) / (16)) ==
-                  (((((st_20.(share)).(globals)).(g_granules)) @ (((v__sroa_0_0_copyload.(poffset)) + (8)) / (16))).[e_ref] :<
-                    ((((((st_20.(share)).(globals)).(g_granules)) @ (((v__sroa_0_0_copyload.(poffset)) + (8)) / (16))).(e_ref)).[e_u_anon_3_0] :<
-                      (((((((st_20.(share)).(globals)).(g_granules)) @ (((v__sroa_0_0_copyload.(poffset)) + (8)) / (16))).(e_ref)).(e_u_anon_3_0)) + (1))))) @ ((v_9.(poffset)) / (16))).(e_ref)).[e_u_anon_3_0] :<
-                  ((g_mapped_addr_set_para
-                    (((((((st_20.(share)).(globals)).(g_granules)) #
-                      (((v__sroa_0_0_copyload.(poffset)) + (8)) / (16)) ==
-                      (((((st_20.(share)).(globals)).(g_granules)) @ (((v__sroa_0_0_copyload.(poffset)) + (8)) / (16))).[e_ref] :<
-                        ((((((st_20.(share)).(globals)).(g_granules)) @ (((v__sroa_0_0_copyload.(poffset)) + (8)) / (16))).(e_ref)).[e_u_anon_3_0] :<
-                          (((((((st_20.(share)).(globals)).(g_granules)) @ (((v__sroa_0_0_copyload.(poffset)) + (8)) / (16))).(e_ref)).(e_u_anon_3_0)) + (1))))) @ ((v_9.(poffset)) / (16))).(e_ref)).(e_u_anon_3_0))
-                    v_2) +
-                    (1)))))).[share].[granule_data] :<
-            (((st_20.(share)).(granule_data)) #
-              (((v_18.(poffset)) + ((8 * (v__sroa_4_0_copyload)))) / (4096)) ==
-              ((((st_20.(share)).(granule_data)) @ (((v_18.(poffset)) + ((8 * (v__sroa_4_0_copyload)))) / (4096))).[g_norm] :<
-                (((((st_20.(share)).(granule_data)) @ (((v_18.(poffset)) + ((8 * (v__sroa_4_0_copyload)))) / (4096))).(g_norm)) #
-                  (((v_18.(poffset)) + ((8 * (v__sroa_4_0_copyload)))) mod (4096)) ==
-                  (test_PTE_Z v_0)))))));
-    (Some (0, st_28)).
-
-  Definition data_create_internal_spec (v_0: Z) (v_1: Ptr) (v_2: Z) (v_3: Ptr) (v_4: Ptr) (v_5: Z) (st: RData) : (option (Z * RData)) :=
+  Definition data_create_internal_spec_abs (v_0_pte: abs_PTE_t) (v_1: Ptr) (v_2: Z) (v_3: Ptr) (v_4: Ptr) (v_5: Z) (st: RData) : (option (Z * RData)) :=
     rely (((((((st.(share)).(granule_data)) @ ((v_4.(poffset)) / (4096))).(g_granule_state)) - (GRANULE_STATE_REC)) = (0)));
     rely (((((v_4.(pbase)) = ("granule_data")) /\ ((((v_4.(poffset)) mod (4096)) = (0)))) /\ (((v_4.(poffset)) >= (0)))));
     rely (((((v_3.(pbase)) = ("granules")) /\ ((((v_3.(poffset)) mod (16)) = (0)))) /\ (((v_3.(poffset)) >= (0)))));
@@ -529,7 +365,7 @@ Section Layer7_Spec.
           ((((abs_tte_read (mkPtr "granule_data" (((rtt_ret.(e_2)).(poffset)) + ((8 * ((rtt_ret.(e_3))))))) st_4).(meta_mem_attr)) =? (0)))))
       then (
         when st_13 == ((granule_lock_spec (rec_to_rd_para v_4 st_4) 2 st_4));
-        when v_11, st_2 == ((memcpy_ns_read_spec (mkPtr "granule_data" (((test_Z_PTE v_0).(meta_PA)).(meta_granule_offset))) (mkPtr "granule_data" (v_3.(poffset))) 4096 st_13));
+        when v_11, st_2 == ((memcpy_ns_read_spec (mkPtr "granule_data" ((v_0_pte.(meta_PA)).(meta_granule_offset))) (mkPtr "granule_data" (v_3.(poffset))) 4096 st_13));
         if v_11
         then (
           when st_18 == ((granule_unlock_spec (rec_to_rd_para v_4 st_4) st_2));
@@ -537,9 +373,7 @@ Section Layer7_Spec.
           then (
             rely ((((rtt_ret.(e_2)).(pbase)) =s ("granules")));
             rely ((((((rtt_ret.(e_2)).(poffset)) + (8)) mod (16)) = (8)));
-            rely (
-              ((("granules" = ("granules")) /\ ((((((test_Z_PTE v_0).(meta_PA)).(meta_granule_offset)) mod (16)) = (0)))) /\
-                (((((test_Z_PTE v_0).(meta_PA)).(meta_granule_offset)) >= (0)))));
+            rely (((("granules" = ("granules")) /\ (((((v_0_pte.(meta_PA)).(meta_granule_offset)) mod (16)) = (0)))) /\ ((((v_0_pte.(meta_PA)).(meta_granule_offset)) >= (0)))));
             when st_29 == (
                 (granule_unlock_spec
                   (rtt_ret.(e_2))
@@ -549,23 +383,23 @@ Section Layer7_Spec.
                       (((((st_18.(share)).(globals)).(g_granules)) @ ((((rtt_ret.(e_2)).(poffset)) + (8)) / (16))).[e_ref] :<
                         ((((((st_18.(share)).(globals)).(g_granules)) @ ((((rtt_ret.(e_2)).(poffset)) + (8)) / (16))).(e_ref)).[e_u_anon_3_0] :<
                           (((((((st_18.(share)).(globals)).(g_granules)) @ ((((rtt_ret.(e_2)).(poffset)) + (8)) / (16))).(e_ref)).(e_u_anon_3_0)) + (1))))) #
-                      ((((test_Z_PTE v_0).(meta_PA)).(meta_granule_offset)) / (16)) ==
+                      (((v_0_pte.(meta_PA)).(meta_granule_offset)) / (16)) ==
                       ((((((st_18.(share)).(globals)).(g_granules)) #
                         ((((rtt_ret.(e_2)).(poffset)) + (8)) / (16)) ==
                         (((((st_18.(share)).(globals)).(g_granules)) @ ((((rtt_ret.(e_2)).(poffset)) + (8)) / (16))).[e_ref] :<
                           ((((((st_18.(share)).(globals)).(g_granules)) @ ((((rtt_ret.(e_2)).(poffset)) + (8)) / (16))).(e_ref)).[e_u_anon_3_0] :<
-                            (((((((st_18.(share)).(globals)).(g_granules)) @ ((((rtt_ret.(e_2)).(poffset)) + (8)) / (16))).(e_ref)).(e_u_anon_3_0)) + (1))))) @ ((((test_Z_PTE v_0).(meta_PA)).(meta_granule_offset)) / (16))).[e_ref] :<
+                            (((((((st_18.(share)).(globals)).(g_granules)) @ ((((rtt_ret.(e_2)).(poffset)) + (8)) / (16))).(e_ref)).(e_u_anon_3_0)) + (1))))) @ (((v_0_pte.(meta_PA)).(meta_granule_offset)) / (16))).[e_ref] :<
                         (((((((st_18.(share)).(globals)).(g_granules)) #
                           ((((rtt_ret.(e_2)).(poffset)) + (8)) / (16)) ==
                           (((((st_18.(share)).(globals)).(g_granules)) @ ((((rtt_ret.(e_2)).(poffset)) + (8)) / (16))).[e_ref] :<
                             ((((((st_18.(share)).(globals)).(g_granules)) @ ((((rtt_ret.(e_2)).(poffset)) + (8)) / (16))).(e_ref)).[e_u_anon_3_0] :<
-                              (((((((st_18.(share)).(globals)).(g_granules)) @ ((((rtt_ret.(e_2)).(poffset)) + (8)) / (16))).(e_ref)).(e_u_anon_3_0)) + (1))))) @ ((((test_Z_PTE v_0).(meta_PA)).(meta_granule_offset)) / (16))).(e_ref)).[e_u_anon_3_0] :<
+                              (((((((st_18.(share)).(globals)).(g_granules)) @ ((((rtt_ret.(e_2)).(poffset)) + (8)) / (16))).(e_ref)).(e_u_anon_3_0)) + (1))))) @ (((v_0_pte.(meta_PA)).(meta_granule_offset)) / (16))).(e_ref)).[e_u_anon_3_0] :<
                           ((g_mapped_addr_set_para
                             (((((((st_18.(share)).(globals)).(g_granules)) #
                               ((((rtt_ret.(e_2)).(poffset)) + (8)) / (16)) ==
                               (((((st_18.(share)).(globals)).(g_granules)) @ ((((rtt_ret.(e_2)).(poffset)) + (8)) / (16))).[e_ref] :<
                                 ((((((st_18.(share)).(globals)).(g_granules)) @ ((((rtt_ret.(e_2)).(poffset)) + (8)) / (16))).(e_ref)).[e_u_anon_3_0] :<
-                                  (((((((st_18.(share)).(globals)).(g_granules)) @ ((((rtt_ret.(e_2)).(poffset)) + (8)) / (16))).(e_ref)).(e_u_anon_3_0)) + (1))))) @ ((((test_Z_PTE v_0).(meta_PA)).(meta_granule_offset)) / (16))).(e_ref)).(e_u_anon_3_0))
+                                  (((((((st_18.(share)).(globals)).(g_granules)) @ ((((rtt_ret.(e_2)).(poffset)) + (8)) / (16))).(e_ref)).(e_u_anon_3_0)) + (1))))) @ (((v_0_pte.(meta_PA)).(meta_granule_offset)) / (16))).(e_ref)).(e_u_anon_3_0))
                             v_2) +
                             (1)))))).[share].[granule_data] :<
                     (((st_18.(share)).(granule_data)) #
@@ -573,15 +407,13 @@ Section Layer7_Spec.
                       ((((st_18.(share)).(granule_data)) @ ((((rtt_ret.(e_2)).(poffset)) + ((8 * ((rtt_ret.(e_3)))))) / (4096))).[g_norm] :<
                         (((((st_18.(share)).(granule_data)) @ ((((rtt_ret.(e_2)).(poffset)) + ((8 * ((rtt_ret.(e_3)))))) / (4096))).(g_norm)) #
                           ((((rtt_ret.(e_2)).(poffset)) + ((8 * ((rtt_ret.(e_3)))))) mod (4096)) ==
-                          (test_PTE_Z (mkabs_PTE_t ((test_Z_PTE v_0).(meta_PA)) 0 0 1))))))));
+                          (test_PTE_Z (mkabs_PTE_t (v_0_pte.(meta_PA)) 0 0 1))))))));
             (Some (0, st_29)))
           else (
             rely ((((rtt_ret.(e_2)).(pbase)) =s ("granules")));
             rely ((((((rtt_ret.(e_2)).(poffset)) + (8)) mod (16)) = (8)));
-            rely (
-              ((("granules" = ("granules")) /\ ((((((test_Z_PTE v_0).(meta_PA)).(meta_granule_offset)) mod (16)) = (0)))) /\
-                (((((test_Z_PTE v_0).(meta_PA)).(meta_granule_offset)) >= (0)))));
-            if (((((((test_Z_PTE v_0).(meta_PA)).(meta_granule_offset)) + (8)) mod (16)) - (8)) =? (0))
+            rely (((("granules" = ("granules")) /\ (((((v_0_pte.(meta_PA)).(meta_granule_offset)) mod (16)) = (0)))) /\ ((((v_0_pte.(meta_PA)).(meta_granule_offset)) >= (0)))));
+            if ((((((v_0_pte.(meta_PA)).(meta_granule_offset)) + (8)) mod (16)) - (8)) =? (0))
             then (
               when st_30 == (
                   (granule_unlock_spec
@@ -592,23 +424,23 @@ Section Layer7_Spec.
                         (((((st_18.(share)).(globals)).(g_granules)) @ ((((rtt_ret.(e_2)).(poffset)) + (8)) / (16))).[e_ref] :<
                           ((((((st_18.(share)).(globals)).(g_granules)) @ ((((rtt_ret.(e_2)).(poffset)) + (8)) / (16))).(e_ref)).[e_u_anon_3_0] :<
                             (((((((st_18.(share)).(globals)).(g_granules)) @ ((((rtt_ret.(e_2)).(poffset)) + (8)) / (16))).(e_ref)).(e_u_anon_3_0)) + (1))))) #
-                        ((((test_Z_PTE v_0).(meta_PA)).(meta_granule_offset)) / (16)) ==
+                        (((v_0_pte.(meta_PA)).(meta_granule_offset)) / (16)) ==
                         ((((((st_18.(share)).(globals)).(g_granules)) #
                           ((((rtt_ret.(e_2)).(poffset)) + (8)) / (16)) ==
                           (((((st_18.(share)).(globals)).(g_granules)) @ ((((rtt_ret.(e_2)).(poffset)) + (8)) / (16))).[e_ref] :<
                             ((((((st_18.(share)).(globals)).(g_granules)) @ ((((rtt_ret.(e_2)).(poffset)) + (8)) / (16))).(e_ref)).[e_u_anon_3_0] :<
-                              (((((((st_18.(share)).(globals)).(g_granules)) @ ((((rtt_ret.(e_2)).(poffset)) + (8)) / (16))).(e_ref)).(e_u_anon_3_0)) + (1))))) @ ((((test_Z_PTE v_0).(meta_PA)).(meta_granule_offset)) / (16))).[e_ref] :<
+                              (((((((st_18.(share)).(globals)).(g_granules)) @ ((((rtt_ret.(e_2)).(poffset)) + (8)) / (16))).(e_ref)).(e_u_anon_3_0)) + (1))))) @ (((v_0_pte.(meta_PA)).(meta_granule_offset)) / (16))).[e_ref] :<
                           (((((((st_18.(share)).(globals)).(g_granules)) #
                             ((((rtt_ret.(e_2)).(poffset)) + (8)) / (16)) ==
                             (((((st_18.(share)).(globals)).(g_granules)) @ ((((rtt_ret.(e_2)).(poffset)) + (8)) / (16))).[e_ref] :<
                               ((((((st_18.(share)).(globals)).(g_granules)) @ ((((rtt_ret.(e_2)).(poffset)) + (8)) / (16))).(e_ref)).[e_u_anon_3_0] :<
-                                (((((((st_18.(share)).(globals)).(g_granules)) @ ((((rtt_ret.(e_2)).(poffset)) + (8)) / (16))).(e_ref)).(e_u_anon_3_0)) + (1))))) @ ((((test_Z_PTE v_0).(meta_PA)).(meta_granule_offset)) / (16))).(e_ref)).[e_u_anon_3_0] :<
+                                (((((((st_18.(share)).(globals)).(g_granules)) @ ((((rtt_ret.(e_2)).(poffset)) + (8)) / (16))).(e_ref)).(e_u_anon_3_0)) + (1))))) @ (((v_0_pte.(meta_PA)).(meta_granule_offset)) / (16))).(e_ref)).[e_u_anon_3_0] :<
                             ((g_mapped_addr_set_para
                               (((((((st_18.(share)).(globals)).(g_granules)) #
                                 ((((rtt_ret.(e_2)).(poffset)) + (8)) / (16)) ==
                                 (((((st_18.(share)).(globals)).(g_granules)) @ ((((rtt_ret.(e_2)).(poffset)) + (8)) / (16))).[e_ref] :<
                                   ((((((st_18.(share)).(globals)).(g_granules)) @ ((((rtt_ret.(e_2)).(poffset)) + (8)) / (16))).(e_ref)).[e_u_anon_3_0] :<
-                                    (((((((st_18.(share)).(globals)).(g_granules)) @ ((((rtt_ret.(e_2)).(poffset)) + (8)) / (16))).(e_ref)).(e_u_anon_3_0)) + (1))))) @ ((((test_Z_PTE v_0).(meta_PA)).(meta_granule_offset)) / (16))).(e_ref)).(e_u_anon_3_0))
+                                    (((((((st_18.(share)).(globals)).(g_granules)) @ ((((rtt_ret.(e_2)).(poffset)) + (8)) / (16))).(e_ref)).(e_u_anon_3_0)) + (1))))) @ (((v_0_pte.(meta_PA)).(meta_granule_offset)) / (16))).(e_ref)).(e_u_anon_3_0))
                               v_2) +
                               (1)))))).[share].[granule_data] :<
                       (((st_18.(share)).(granule_data)) #
@@ -616,11 +448,11 @@ Section Layer7_Spec.
                         ((((st_18.(share)).(granule_data)) @ ((((rtt_ret.(e_2)).(poffset)) + ((8 * ((rtt_ret.(e_3)))))) / (4096))).[g_norm] :<
                           (((((st_18.(share)).(granule_data)) @ ((((rtt_ret.(e_2)).(poffset)) + ((8 * ((rtt_ret.(e_3)))))) / (4096))).(g_norm)) #
                             ((((rtt_ret.(e_2)).(poffset)) + ((8 * ((rtt_ret.(e_3)))))) mod (4096)) ==
-                            (test_PTE_Z (mkabs_PTE_t ((test_Z_PTE v_0).(meta_PA)) 0 0 3))))))));
+                            (test_PTE_Z (mkabs_PTE_t (v_0_pte.(meta_PA)) 0 0 3))))))));
               (Some (0, st_30)))
             else None))
         else (
-          when v_33, st_18 == ((memset_spec (mkPtr "granule_data" (((test_Z_PTE v_0).(meta_PA)).(meta_granule_offset))) 0 4096 st_2));
+          when v_33, st_18 == ((memset_spec (mkPtr "granule_data" ((v_0_pte.(meta_PA)).(meta_granule_offset))) 0 4096 st_2));
           when st_19 == ((granule_unlock_spec (rec_to_rd_para v_4 st_4) st_18));
           when st_21 == ((granule_unlock_spec (rtt_ret.(e_2)) st_19));
           (Some ((pack_struct_return_code_para (make_return_code_para 1)), st_21))))
@@ -630,6 +462,20 @@ Section Layer7_Spec.
     else (
       when st_8 == ((granule_unlock_spec (rtt_ret.(e_2)) st_4));
       (Some ((pack_struct_return_code_para (make_return_code_para 8)), st_8))).
+
+  Definition granule_unlock_transition_spec (v_0: Ptr) (v_1: Z) (st: RData) : (option RData) :=
+    rely (((((v_0.(pbase)) = ("granules")) /\ ((((v_0.(poffset)) mod (16)) = (0)))) /\ (((v_0.(poffset)) >= (0)))));
+    when st_1 == (
+        (granule_unlock_spec
+          v_0
+          (st.[share].[globals].[g_granules] :<
+            ((((st.(share)).(globals)).(g_granules)) #
+              ((v_0.(poffset)) / (16)) ==
+              (((((st.(share)).(globals)).(g_granules)) @ ((v_0.(poffset)) / (16))).[e_state_s_granule] :< v_1)))));
+    (Some st_1).
+
+  Definition data_create_internal_spec (v_0: Z) (v_1: Ptr) (v_2: Z) (v_3: Ptr) (v_4: Ptr) (v_5: Z) (st: RData) : (option (Z * RData)) :=
+    None.
 
 End Layer7_Spec.
 
@@ -642,8 +488,6 @@ End Layer7_Spec.
 #[global] Hint Unfold smc_granule_any_to_ns_spec_abs: spec.
 #[global] Hint Unfold granule_pa_to_va_spec_abs: spec.
 #[global] Hint Unfold ns_buffer_read_spec_abs: spec.
-#[global] Hint Unfold data_create_internal_0: spec.
-#[global] Hint Unfold data_create_internal_1: spec.
-#[global] Hint Unfold data_create_internal_2: spec.
-#[global] Hint Unfold data_create_internal_3: spec.
+#[global] Hint Unfold data_create_internal_spec_abs: spec.
+#[global] Hint Unfold granule_unlock_transition_spec: spec.
 #[global] Hint Unfold data_create_internal_spec: spec.
