container/coq/pointer/Layer7/granule_unlock_transition/LowSpec.v
@@ -2,8 +2,6 @@ Require Import Code.
 Require Import CommonDeps.
 Require Import DataTypes.
 Require Import GlobalDefs.
-Require Import Layer5.Spec.
-Require Import Layer6.Spec.
 
 Local Open Scope string_scope.
 Local Open Scope Z_scope.
@@ -13,11 +11,15 @@ Section Layer7_granule_unlock_transition_LowSpec.
   Context `{int_ptr: IntPtrCast}.
 
   Definition granule_unlock_transition_spec_low (v_0: Ptr) (v_1: Z) (st: RData) : (option RData) :=
-    rely (((((((v_0.(pbase)) = ("granules")) /\ ((((v_0.(poffset)) mod (16)) = (0)))) /\ (((v_0.(poffset)) >= (0)))) /\ ((v_1 >= (0)))) /\ ((v_1 <= (6)))));
-    rely (((((((v_0.(pbase)) = ("granules")) /\ ((((v_0.(poffset)) mod (16)) = (0)))) /\ (((v_0.(poffset)) >= (0)))) /\ ((v_1 >= (0)))) /\ ((v_1 <= (6)))));
-    when st_1 == ((store_RData 4 (mkPtr (v_0.(pbase)) ((v_0.(poffset)) + (4))) v_1 st));
-    when st_3 == ((granule_unlock_spec v_0 st_1));
-    (Some st_3).
+    rely (((((v_0.(pbase)) = ("granules")) /\ ((((v_0.(poffset)) mod (16)) = (0)))) /\ (((v_0.(poffset)) >= (0)))));
+    when st_1 == (
+        (granule_unlock_spec
+          v_0
+          (st.[share].[globals].[g_granules] :<
+            ((((st.(share)).(globals)).(g_granules)) #
+              ((v_0.(poffset)) / (16)) ==
+              (((((st.(share)).(globals)).(g_granules)) @ ((v_0.(poffset)) / (16))).[e_state_s_granule] :< v_1)))));
+    (Some st_1).
 
 End Layer7_granule_unlock_transition_LowSpec.
 
